Typing for Assign, some more helper functions

Semantics.thy
@@ -324,10 +324,17 @@ definition ty_includes :: "ty_env \<Rightarrow> heap_ty \<Rightarrow> instanc \<
 definition ty_excludes :: "ty_env \<Rightarrow> heap_ty \<Rightarrow> instanc \<Rightarrow> bool" where
   "ty_excludes \<Gamma> \<tau> i = (\<forall>\<epsilon>. \<epsilon> \<TTurnstile> \<Gamma> \<longrightarrow> (\<forall>h \<in> \<lbrakk>\<tau> in \<epsilon>\<rbrakk>\<^sub>t. i \<notin> heap_dom h))"
 
+text\<open>Helpers for constructing various predicate formulas.\<close>
+
 nominal_function heap_instance_eq :: "header_table \<Rightarrow> var \<Rightarrow> var \<Rightarrow> formula" where
-  "heap_instance_eq HT x y = foldr (\<lambda>(i, ht) \<phi>. (let hl = header_length ht in
-    And (Eq (Slice (SlInstance x i) 0 hl) (Slice (SlInstance y i) 0 hl)) \<phi>)) HT FTrue"
+  "heap_instance_eq ((i,ht)#HT) x y = (let hl = header_length ht in
+   And (Eq (Slice (SlInstance x i) 0 hl) (Slice (SlInstance y i) 0 hl))
+       (heap_instance_eq HT x y))" |
+  "heap_instance_eq [] x y = FTrue"
   subgoal by (auto simp add: eqvt_def heap_instance_eq_graph_aux_def Let_def)
+  subgoal by (simp)
+  apply (clarify)
+  subgoal for P HT x y by (rule list.exhaust) (auto)
   apply (auto)
 done
 nominal_termination (eqvt)
@@ -342,6 +349,63 @@ nominal_function heap_eq :: "header_table \<Rightarrow> var \<Rightarrow> var \<
 done
 nominal_termination (eqvt)
   by lexicographic_order
+
+nominal_function instances_eq_except :: "header_table \<Rightarrow> instanc \<Rightarrow> var \<Rightarrow> var \<Rightarrow> formula" where
+  "instances_eq_except HT i x y = heap_instance_eq [(k,ht)\<leftarrow>HT. k \<noteq> i] x y"
+  subgoal by (auto simp add: eqvt_def instances_eq_except_graph_aux_def Let_def)
+  apply (auto)
+done
+nominal_termination (eqvt)
+  by lexicographic_order
+
+nominal_function fields_eq_except_helper :: "field list \<Rightarrow> instanc \<Rightarrow> field_name \<Rightarrow> var \<Rightarrow> var \<Rightarrow> formula"
+where
+  "fields_eq_except_helper ((Field f _)#fs) i g x y = (let rem = fields_eq_except_helper fs i g x y in
+    let this = if f = g then FTrue else let (n, m) = field_list_to_range fs f in
+      Eq (Slice (SlInstance x i) n m) (Slice (SlInstance y i) n m) in
+    And this rem)" |
+  "fields_eq_except_helper [] _ _ _ _ = FTrue"
+  subgoal by (auto simp add: eqvt_def fields_eq_except_helper_graph_aux_def)
+  subgoal by (simp)
+  apply (clarify)
+  subgoal for P fs i g x y
+    apply (rule list.exhaust) apply (auto)
+    by (rule field.exhaust) (auto)
+  apply (auto)
+done
+nominal_termination (eqvt)
+  by lexicographic_order
+
+nominal_function fields_eq_except :: "header_type \<Rightarrow> instanc \<Rightarrow> field_name \<Rightarrow> var \<Rightarrow> var \<Rightarrow> formula"
+where
+  "fields_eq_except (HeaderType _ fs) i g x y = fields_eq_except_helper fs i g x y"
+  subgoal by (auto simp add: eqvt_def fields_eq_except_graph_aux_def)
+  subgoal by (simp)
+  apply (clarify)
+  subgoal for P ht i g x y by (rule header_type.exhaust) (auto)
+  apply (auto)
+done
+nominal_termination (eqvt)
+  by lexicographic_order
+
+(*
+  "fields_eq_except (HeaderType _ (f#fs)) i g x y = (let rem = fields_eq_except 
+(if f = g then FTrue else
+    let (n, m) = field_list_to_range fs f in
+      And (Eq (Slice (SlInstance x i) n m) (Slice (SlInstance y i) n m))
+          fields_eq_except 
+
+nominal_function fields_eq_except :: "header_type \<Rightarrow> instanc \<Rightarrow> field_name \<Rightarrow> var \<Rightarrow> var \<Rightarrow> formula"
+where
+  "fields_eq_except ht i f x y = (case ht of (HeaderType _ fs) \<Rightarrow> foldr (\<lambda>g \<phi>.
+    (let (n, m) = header_field_to_range ht g in
+      And (Eq (Slice (SlInstance x i) n m) (Slice (SlInstance y i) n m)) \<phi>))
+    [g. gf\<leftarrow>fs, (case gf of (Field g _) \<Rightarrow> g \<noteq> f)] FTrue)"
+  subgoal apply (auto simp add: eqvt_def fields_eq_except_graph_aux_def Let_def lfp_eqvt )
+find_theorems "_ \<bullet> (\<lambda>_. _)_"
+
+thm eqvts
+*)
 
 (* TODO: I can't get the prios for this and ty_env_add_heap (";") such that this is not ambigious *)
 inductive exp_typing :: "ty_env \<Rightarrow> exp \<Rightarrow> base_ty \<Rightarrow> bool"
@@ -393,5 +457,19 @@ where
                    HT, \<Gamma> \<turnstile> c\<^sub>1 : ((x : Refinement y \<tau>\<^sub>1 \<phi>[y/var_heap]\<^sub>f) \<rightarrow> \<tau>12);
                    HT, \<Gamma> \<turnstile> c\<^sub>2 : ((x : Refinement y \<tau>\<^sub>1 (Not \<phi>[y/var_heap]\<^sub>f)) \<rightarrow> \<tau>22) \<rbrakk>
                 \<Longrightarrow> HT, \<Gamma> \<turnstile> (If \<phi> c\<^sub>1 c\<^sub>2) : ((x : \<tau>\<^sub>1) \<rightarrow>
-                  Choice (Refinement y \<tau>12 \<phi>[x/var_heap]\<^sub>f) (Refinement y \<tau>22 (Not \<phi>[x/heap]\<^sub>f)))"
+                  Choice (Refinement y \<tau>12 \<phi>[x/var_heap]\<^sub>f) (Refinement y \<tau>22 (Not \<phi>[x/heap]\<^sub>f)))" |
+                (* Ignoring the F(i,f) = BV premise here. The paper never mentions it, the thesis
+                   seems to say it would be useful for potentially more fine-grained checking as
+                   an extension, but it's not actually used yet. *)
+  TC_Assign:    "\<lbrakk> ty_includes \<Gamma> \<tau>\<^sub>1 i;
+                   (\<Gamma>; \<tau>\<^sub>1) \<turnstile>\<^sub>e e : BV;
+                   \<phi>pkt = And (Eq (Packet y PktIn) (Packet x PktIn))
+                              (Eq (Packet y PktOut) (Packet x PktOut));
+                   \<phi>i = instances_eq_except HT i y x;
+                   map_of HT i = Some ht;
+                   header_field_to_range ht f = (n, m);
+                   \<phi>f = fields_eq_except ht f i y x;
+                   \<phi>feq = Eq (Slice (SlInstance y i) n m) e[x/heap]\<^sub>e \<rbrakk>
+                \<Longrightarrow> HT, \<Gamma> \<turnstile> (Assign i f e) : ((x : \<tau>\<^sub>1) \<rightarrow> Refinement y Top
+                      (And \<phi>pkt (And \<phi>i (And \<phi>f \<phi>feq))))"
 end
